1. $n \in \mathbb{N}$ s.t $2<n \space\and\space2\mid n$. Show that for any $\sigma \in A_n$, there are $\tau_1,...,\tau_{n-2}\in S_n$ for which $\sigma=\tau_1\cdot\cdot\cdot\tau_{n-2}$.

   <u>Proof</u>

   By induction on $n$.

   The statement is true for $n=4$.

   Assume the statement is true for any $2\mid k<n$, and we will prove it for $n$.

   Pick some $\sigma \in A_n$.

   * If $\sigma \in A_{n-2}$, then by the induction hypothesis: $\sigma=\tau_1\cdot\cdot\cdot\tau_{n-4}=\tau_1\cdot\cdot\cdot\tau_{n-4}(n,n-1)(n, n-1)$. 

     Thus the statement holds.

   * If $\sigma \notin A_{n-2}$ then $\sigma=(a_1,...,a_t)(b_1,...,b_l)...(...)$.

     Without loss of generality, we can assume 3 cases:

     <u>Case 1</u>: $n\in (a_1,...,a_t), n-1\notin (a_1,...,a_t),(b_1,...,b_l)$

     <u>Case 2</u>: $n\in (a_1,...,a_t), n-1\in (b_1,...,b_l)$

     <u>Case 3</u>: $n,n-1\in (a_1,...,a_t)$

     

     We prove <u>Case 1</u>, and leave the rest for the reader.

     Assume without loss of generality $a_t=n$.

     $\sigma=(a_1,...,a_{t-2})(b_1,...,b_l)...(...)(a_{t-2},a_{t-1})(a_{t-1},a_t)$.

     $\sigma^{'}=(a_1,...,a_{t-2})(b_1,...,b_l)...(...) \in A_{n-2}$.

     $\sigma=\sigma^{'}(a_{t-2},a_{t-1})(a_{t-1},a_t)$.

     We use the induction hypothesis on $\sigma^{'}$....

   ###### Note

   The same proof won't work for $2\nmid n$. The base case of the induction fails on $n=3$.

   

2. $\varphi:D_n \mapsto G$ epi-morphism for some $3\le n$, $2\nmid n$.

   <u>Proof</u>

   $G\cong D_n/ker(\varphi)$, and since n is odd, $ker(\varphi) = [\sigma^k]$ for some $k\mid n$.

   Define a homomorphism $\eta:D_n \mapsto D_{\frac{n}{k}}$ by:

   * $(\sigma^i)\eta=\sigma^{i(mod\frac{n}{k})}$.
   * $(\sigma^i\tau)\eta=\sigma^{i(mod\frac{n}{k})}\tau$

   Check $\eta$ is an epi-morphism, and $ker(\eta) = [\sigma^k] = ker(\varphi)$.

   Then we have $D_n/ker(\varphi)\cong G \cong D_n/ker(\eta) \cong Im(\eta) = D_{\frac{n}{k}}$.